src/Ex/Msi/MsiImp.v
@@ -1,0 +1,223 @@
+Require Import Bool Vector List String Peano_dec Lia.
+Require Import Common FMap HVector IndexSupport Syntax Semantics.
+Require Import Topology RqRsTopo.
+Require Import RqRsLang. Import RqRsNotations.
+
+Require Import Ex.Spec Ex.SpecInds Ex.Template Ex.RuleTransform Ex.Msi.
+Require Import Ex.Msi.Msi.
+
+Set Implicit Arguments.
+
+Local Open Scope list.
+Local Open Scope hvec.
+Local Open Scope fmap.
+
+Existing Instance Msi.ImplOStateIfc.
+
+Section System.
+  Variable (tr: tree).
+  Hypothesis (Htr: tr <> Node nil).
+
+  Let topo := fst (tree2Topo tr 0).
+  Let cifc := snd (tree2Topo tr 0).
+
+  Section Rules.
+    Variables (oidx cidx: IdxT).
+
+    (** L1 caches remain the same. *)
+
+    Section Li.
+
+      Definition liDownSRsUpDownOne: Rule :=
+        rule.rsuo[0~>4~>0~~cidx]
+        :accepts msiDownRsS
+        :holding msiRqS
+        :from cidx.
+
+      Definition liDownSRsUpDownRel: Rule :=
+        rule.rsro[0~>4~>1]
+        :holding msiRqS
+        :requires (fun _ _ _ => True)
+        :transition
+           (!|ost, idm, rq, rsbTo|
+            --> (ost +#[owned <- true]
+                     +#[val <- msg_value (valOf idm)]
+                     +#[status <- msiS]
+                     +#[dir <- setDirS [objIdxOf rsbTo; objIdxOf (idOf idm)]],
+                 <| msiRsS; msg_value (valOf idm) |>)).
+
+      Definition liDownSRsUpUpOne: Rule :=
+        rule.rsuo[0~>7~>0~~cidx]
+        :accepts msiDownRsS
+        :holding msiDownRqS
+        :from cidx.
+
+      Definition liDownSRsUpUpRel: Rule :=
+        rule.rsro[0~>7~>1]
+        :holding msiDownRqS
+        :requires (fun _ _ _ => True)
+        :transition
+           (!|ost, idm, rq, rsbTo|
+            --> (ost +#[val <- msg_value (valOf idm)]
+                     +#[owned <- false]
+                     +#[status <- msiS]
+                     +#[dir <- setDirS [objIdxOf (idOf idm)]],
+                 <| msiDownRsS; msg_value (valOf idm) |>)).
+
+      Definition liDownIRsUpDownSOne: Rule :=
+        rule.rsuo[1~>6~>0~>0~~cidx]
+        :accepts msiDownRsIS
+        :holding msiRqM
+        :from cidx.
+
+      Definition liDownIRsUpDownMOne: Rule :=
+        rule.rsuo[1~>6~>0~>1~~cidx]
+        :accepts msiDownRsIM
+        :holding msiRqM
+        :from cidx.
+
+      Definition liDownIRsUpDownRel: Rule :=
+        rule.rsr[1~>6~>1]
+        :holding msiRqM
+        :requires (fun _ _ _ => True)
+        :transition
+           (!|ost, mins, rq, rsbTo|
+            --> (ost +#[owned <- false]
+                     +#[status <- msiI]
+                     +#[dir <- setDirM (objIdxOf rsbTo)],
+                 <| msiRsM; O |>)).
+
+      Definition liDownIRsUpUpSOne: Rule :=
+        rule.rsuo[1~>10~>0~>0~~cidx]
+        :accepts msiDownRsIS
+        :holding msiDownRqIS
+        :from cidx.
+
+      Definition liDownIRsUpUpMOne: Rule :=
+        rule.rsuo[1~>10~>0~>1~~cidx]
+        :accepts msiDownRsIM
+        :holding msiDownRqIM
+        :from cidx.
+
+      Definition liDownIRsUpUpSRel: Rule :=
+        rule.rsr[1~>10~>1~>0]
+        :holding msiDownRqIS
+        :requires (fun _ _ _ => True)
+        :transition
+           (!|ost, mins, rq, rsbTo|
+            --> (ost +#[owned <- false]
+                     +#[status <- msiI]
+                     +#[dir <- setDirI],
+                 <| msiDownRsIS; O |>)).
+
+      Definition liDownIRsUpUpMRel: Rule :=
+        rule.rsr[1~>10~>1~>1]
+        :holding msiDownRqIM
+        :requires (fun _ _ _ => True)
+        :transition
+           (!|ost, mins, rq, rsbTo|
+            --> (ost +#[owned <- false]
+                     +#[status <- msiI]
+                     +#[dir <- setDirI],
+                 <| msiDownRsIM; O |>)).
+
+    End Li.
+
+  End Rules.
+
+  Section Objects.
+    Variable (oidx: IdxT).
+
+    Definition liRulesFromChild (cidx: IdxT): list Rule :=
+      (Msi.liRulesFromChild tr oidx cidx)
+        ++ [liDownSRsUpDownOne cidx; liDownSRsUpUpOne cidx;
+           liDownIRsUpDownSOne cidx; liDownIRsUpDownMOne cidx;
+           liDownIRsUpUpSOne cidx; liDownIRsUpUpMOne cidx].
+
+    Definition liRulesFromChildren (coinds: list IdxT): list Rule :=
+      List.concat (map liRulesFromChild coinds).
+
+    Hint Unfold liRulesFromChild liRulesFromChildren: RuleConds.
+
+    Ltac disc_child_inds_disj :=
+      pose proof (tree2Topo_TreeTopo tr 0);
+      try match goal with
+          | [Hn: ?n1 <> ?n2,
+                 H1: nth_error (subtreeChildrenIndsOf ?topo ?sidx) ?n1 = Some _,
+                     H2: nth_error (subtreeChildrenIndsOf ?topo ?sidx) ?n2 = Some _ |- _] =>
+            eapply TreeTopo_children_inds_disj in Hn; eauto; destruct Hn
+          end.
+
+    Program Definition li: Object :=
+      {| obj_idx := oidx;
+         obj_rules :=
+           (liRulesFromChildren (subtreeChildrenIndsOf topo oidx))
+             (** rules involved with [GetS] *)
+             ++ [liGetSRsDownDown; liDownSRsUpDownRel;
+                liDownSImm oidx; liDownSRqDownDownM tr oidx; liDownSRsUpUpRel]
+             (** rules involved with [GetM] *)
+             ++ [liGetMRsDownDownDirI; liGetMRsDownRqDownDirS tr oidx; liDownIRsUpDownRel;
+                liDownIImmS oidx; liDownIImmM oidx;
+                liDownIRqDownDownDirS tr oidx; liDownIRqDownDownDirM tr oidx;
+                liDownIRsUpUpSRel; liDownIRsUpUpMRel]
+             (** rules involved with [Put] *)
+             ++ [liInvRqUpUp oidx; liInvRqUpUpWB oidx; liInvRsDownDown; liPushImm];
+         obj_rules_valid := _ |}.
+    Next Obligation.
+      solve_inds_NoDup disc_child_inds_disj.
+    Qed.
+
+    Definition memRulesFromChild (cidx: IdxT): list Rule :=
+      (Msi.memRulesFromChild tr oidx cidx)
+        ++ [liDownSRsUpDownOne cidx; liDownIRsUpDownSOne cidx; liDownIRsUpDownMOne cidx].
+
+    Definition memRulesFromChildren (coinds: list IdxT): list Rule :=
+      List.concat (map memRulesFromChild coinds).
+
+    Hint Unfold memRulesFromChild memRulesFromChildren: RuleConds.
+
+    Program Definition mem: Object :=
+      {| obj_idx := oidx;
+         obj_rules :=
+           (memRulesFromChildren (subtreeChildrenIndsOf topo oidx))
+             ++ [liDownSRsUpDownRel; liDownIRsUpDownRel];
+         obj_rules_valid := _ |}.
+    Next Obligation.
+      solve_inds_NoDup disc_child_inds_disj.
+    Qed.
+
+  End Objects.
+
+  Program Definition impl: System :=
+    {| sys_objs :=
+         ((mem (rootOf topo) :: map li (tl cifc.(c_li_indices)))
+            ++ map l1 cifc.(c_l1_indices));
+       sys_oinds_valid := _;
+       sys_minds := cifc.(c_minds);
+       sys_merqs := cifc.(c_merqs);
+       sys_merss := cifc.(c_merss);
+       sys_msg_inds_valid := _;
+       sys_oss_inits := implOStatesInit tr;
+       sys_orqs_inits := implORqsInit tr |}.
+  Next Obligation.
+    unfold mem, li, l1.
+    rewrite map_app.
+    do 2 rewrite map_trans.
+    do 2 rewrite map_id.
+    unfold topo, cifc.
+    rewrite app_comm_cons.
+    rewrite <-c_li_indices_head_rootOf by assumption.
+    apply tree2Topo_WfCIfc.
+  Qed.
+  Next Obligation.
+    apply tree2Topo_WfCIfc.
+  Qed.
+
+End System.
+
+Hint Unfold liDownSRsUpDownOne liDownSRsUpDownRel
+     liDownSRsUpUpOne liDownSRsUpUpRel
+     liDownIRsUpDownSOne liDownIRsUpDownMOne
+     liDownIRsUpDownRel
+     liDownIRsUpUpSOne liDownIRsUpUpMOne
+     liDownIRsUpUpSRel liDownIRsUpUpMRel: MsiRules.
